CaseStudy/ifc_SO/Testing/SingleStateArb.v
@@ -15,12 +15,14 @@ Require Import Printing.
    create (inefficient) instances for a single machine *)
 
 (* Generates an SSNI-oriented single machine state *)
+Definition genState {Gen : Type -> Type} `{GenMonad Gen} : Gen State := 
+  bindGen gen_variation_state (fun v =>
+  let '(Var _ st _) := v in 
+  returnGen st).
+
 Instance arbState : Arbitrary State :=
 {| 
-  arbitrary := 
-    bindGen gen_variation_state (fun v =>
-    let '(Var _ st _) := v in 
-    returnGen st);
+  arbitrary := @genState ;  
   shrink x := 
     let '(St _ _ prins _ _ _) := x in
     let all := shrinkVState (Var prins x x) in
